SStructTT/SStruct/Erasure/Substitution.lean
@@ -9,34 +9,34 @@ variable {Srt : Type} [ord : SrtOrder Srt]
 inductive AgreeSubst :
   (Var -> SStruct.Tm Srt) ->
   (Var -> Erasure.Tm Srt) ->
-  Static.Ctx Srt -> Dynamic.Ctx Srt ->
-  Static.Ctx Srt -> Dynamic.Ctx Srt -> Prop
+  Dynamic.Ctx Srt ->
+  Dynamic.Ctx Srt -> Prop
 where
   | nil {σ σ'} :
-    AgreeSubst σ σ' [] [] [] []
-  | cons {Γ Γ' Δ Δ' A} r {s i σ σ'} :
-    Γ ⊢ A : .srt s i ->
-    AgreeSubst σ σ' Γ Δ Γ' Δ' ->
-    AgreeSubst (up σ) (up σ') (A :: Γ) (A :⟨r, s⟩ Δ) (A.[σ] :: Γ') (A.[σ] :⟨r, s⟩ Δ')
-  | intro_im {Γ Γ' Δ Δ' A m m' s σ σ'} :
-    Γ' ⊢ m : A.[σ] ->
-    AgreeSubst σ σ' Γ Δ Γ' Δ' ->
-    AgreeSubst (m .: σ) (m' .: σ') (A :: Γ) (A :⟨.im, s⟩ Δ) Γ' Δ'
-  | intro_ex {Γ Γ' Δ Δ' Δa Δb A m m' s σ σ'} :
+    AgreeSubst σ σ' [] []
+  | cons {Δ Δ' : Ctx Srt} {A s i σ σ'} r :
+    Δ.static ⊢ A : .srt s i ->
+    AgreeSubst σ σ' Δ Δ' ->
+    AgreeSubst (up σ) (up σ') (A :⟨r, s⟩ Δ) (A.[σ] :⟨r, s⟩ Δ')
+  | intro_im {Δ Δ' : Ctx Srt} {A m m' s σ σ'} :
+    Δ'.static ⊢ m : A.[σ] ->
+    AgreeSubst σ σ' Δ Δ' ->
+    AgreeSubst (m .: σ) (m' .: σ') (A :⟨.im, s⟩ Δ) Δ'
+  | intro_ex {Δ Δ' Δa Δb : Ctx Srt} {A m m' s σ σ'} :
     Merge Δa Δb Δ' ->
     Lower Δa s ->
-    Γ' ;; Δa ⊢ m ▷ m' : A.[σ] ->
-    AgreeSubst σ σ' Γ Δ Γ' Δb ->
-    AgreeSubst (m .: σ) (m' .: σ') (A :: Γ) (A :⟨.ex, s⟩ Δ) Γ' Δ'
-  | conv {Γ Γ' Δ Δ' A B r s i σ σ'} :
+    Δa ⊢ m ▷ m' :: A.[σ] ->
+    AgreeSubst σ σ' Δ Δb ->
+    AgreeSubst (m .: σ) (m' .: σ') (A :⟨.ex, s⟩ Δ) Δ'
+  | conv {Δ Δ' : Ctx Srt} {A B r s i σ σ'} :
     A === B ->
-    Γ ⊢ B : .srt s i ->
-    Γ' ⊢ B.[shift 1].[σ] : .srt s i ->
-    AgreeSubst σ σ' (A :: Γ) (A :⟨r, s⟩ Δ) Γ' Δ' ->
-    AgreeSubst σ σ' (B :: Γ) (B :⟨r, s⟩ Δ) Γ' Δ'
+    Δ.static ⊢ B : .srt s i ->
+    Δ'.static ⊢ B.[shift 1].[σ] : .srt s i ->
+    AgreeSubst σ σ' (A :⟨r, s⟩ Δ) Δ' ->
+    AgreeSubst σ σ' (B :⟨r, s⟩ Δ) Δ'
 
-lemma AgreeSubst.toDynamic {Γ Γ'} {Δ Δ' : Ctx Srt} {σ σ'} :
-    Erasure.AgreeSubst σ σ' Γ Δ Γ' Δ' -> Dynamic.AgreeSubst σ Γ Δ Γ' Δ' := by
+lemma AgreeSubst.toDynamic {Δ Δ' : Ctx Srt} {σ σ'} :
+    Erasure.AgreeSubst σ σ' Δ Δ' -> Dynamic.AgreeSubst σ Δ Δ' := by
   intro agr
   induction agr <;> try aesop (rule_sets := [subst])
   case cons => constructor <;> assumption
@@ -45,12 +45,12 @@ lemma AgreeSubst.toDynamic {Γ Γ'} {Δ Δ' : Ctx Srt} {σ σ'} :
     constructor <;> try assumption
     apply tym.toDynamic
 
-lemma AgreeSubst.toStatic {Γ Γ'} {Δ Δ' : Ctx Srt} {σ σ'} :
-    Erasure.AgreeSubst σ σ' Γ Δ Γ' Δ' -> Static.AgreeSubst σ Γ Γ' := by
+lemma AgreeSubst.toStatic {Δ Δ' : Ctx Srt} {σ σ'} :
+    Erasure.AgreeSubst σ σ' Δ Δ' -> Static.AgreeSubst σ Δ.static Δ'.static := by
   intro agr; apply agr.toDynamic.toStatic
 
 @[aesop safe (rule_sets := [subst])]
-lemma AgreeSubst.refl {Γ} {Δ : Ctx Srt} : Γ ;; Δ ⊢ -> AgreeSubst ids ids Γ Δ Γ Δ := by
+lemma AgreeSubst.refl {Δ : Ctx Srt} : Δ ⊢ -> AgreeSubst ids ids Δ Δ := by
   intro wf; induction wf
   all_goals try trivial
   case nil => constructor
@@ -59,21 +59,21 @@ lemma AgreeSubst.refl {Γ} {Δ : Ctx Srt} : Γ ;; Δ ⊢ -> AgreeSubst ids ids �
     asimp at agr; assumption
 
 @[aesop safe (rule_sets := [subst])]
-lemma AgreeSubst.implicit_image {Γ Γ'} {Δ Δ' : Ctx Srt} {σ σ'} :
-    AgreeSubst σ σ' Γ Δ Γ' Δ' -> Implicit Δ -> Implicit Δ' := by
+lemma AgreeSubst.implicit_image {Δ Δ' : Ctx Srt} {σ σ'} :
+    AgreeSubst σ σ' Δ Δ' -> Implicit Δ -> Implicit Δ' := by
   intro agr; apply agr.toDynamic.implicit_image
 
 @[aesop safe (rule_sets := [subst])]
-lemma AgreeSubst.lower_image {Γ Γ'} {Δ Δ' : Ctx Srt} {s σ σ'} :
-    AgreeSubst σ σ' Γ Δ Γ' Δ' -> Lower Δ s -> Lower Δ' s := by
+lemma AgreeSubst.lower_image {Δ Δ' : Ctx Srt} {s σ σ'} :
+    AgreeSubst σ σ' Δ Δ' -> Lower Δ s -> Lower Δ' s := by
   intro agr; apply agr.toDynamic.lower_image
 
-lemma AgreeSubst.has {Γ Γ'} {Δ Δ' : Ctx Srt} {A x s σ σ'} :
-    AgreeSubst σ σ' Γ Δ Γ' Δ' -> Γ' ;; Δ' ⊢ ->
-    Has Δ x s A -> Γ' ;; Δ' ⊢ (σ x) ▷ (σ' x) : A.[σ] := by
+lemma AgreeSubst.has {Δ Δ' : Ctx Srt} {A x s σ σ'} :
+    AgreeSubst σ σ' Δ Δ' -> Δ' ⊢ ->
+    Has Δ x s A -> Δ' ⊢ (σ x) ▷ (σ' x) :: A.[σ] := by
   intro agr wf hs; induction agr generalizing x A
   case nil => cases hs
-  case cons A r s i σ σ' tyA agr ih =>
+  case cons A s i σ σ' r tyA agr ih =>
     cases r with
     | ex =>
       rcases hs with ⟨im⟩; asimp
@@ -108,42 +108,52 @@ lemma AgreeSubst.has {Γ Γ'} {Δ Δ' : Ctx Srt} {A x s σ σ'} :
       . apply ih wf; constructor; assumption
       . assumption
 
-lemma AgreeSubst.split {Γ Γ'} {Δ Δ' Δa Δb : Ctx Srt} {σ σ'} :
-    AgreeSubst σ σ' Γ Δ Γ' Δ' -> Merge Δa Δb Δ ->
+lemma AgreeSubst.split {Δ Δ' Δa Δb : Ctx Srt} {σ σ'} :
+    AgreeSubst σ σ' Δ Δ' -> Merge Δa Δb Δ ->
     ∃ Δa' Δb',
       Merge Δa' Δb' Δ' ∧
-      AgreeSubst σ σ' Γ Δa Γ' Δa' ∧
-      AgreeSubst σ σ' Γ Δb Γ' Δb' := by
+      AgreeSubst σ σ' Δa Δa' ∧
+      AgreeSubst σ σ' Δb Δb' := by
   intro agr mrg; induction agr generalizing Δa Δb
   case nil =>
     cases mrg; existsi [], []
     aesop (rule_sets := [subst])
-  case cons A r s i σ σ' tyA agr ih =>
+  case cons A s i σ σ' r tyA agr ih =>
     cases mrg with
     | contra _ _ h mrg =>
-      have ⟨Δa', Δb', mrg, agr1, agr2⟩ := ih mrg
+      have ⟨Δa', Δb', _, agr1, agr2⟩ := ih mrg
       existsi A.[σ] :⟨.ex, s⟩ Δa', A.[σ] :⟨.ex, s⟩ Δb'; and_intros
-      all_goals constructor <;> assumption
+      all_goals constructor <;> try assumption
+      rw[<-mrg.static]; assumption
+      rw[<-mrg.sym.static]; assumption
     | left _ _ mrg =>
-      have ⟨Δa', Δb', mrg, agr1, agr2⟩ := ih mrg
+      have ⟨Δa', Δb', _, agr1, agr2⟩ := ih mrg
       existsi A.[σ] :⟨.ex, s⟩ Δa', A.[σ] :⟨.im, s⟩ Δb'; and_intros
-      all_goals constructor <;> assumption
+      all_goals constructor <;> try assumption
+      rw[<-mrg.static]; assumption
+      rw[<-mrg.sym.static]; assumption
     | right _ _ mrg =>
-      have ⟨Δa', Δb', mrg, agr1, agr2⟩ := ih mrg
+      have ⟨Δa', Δb', _, agr1, agr2⟩ := ih mrg
       existsi A.[σ] :⟨.im, s⟩ Δa', A.[σ] :⟨.ex, s⟩ Δb'; and_intros
-      all_goals constructor <;> assumption
+      all_goals constructor <;> try assumption
+      rw[<-mrg.static]; assumption
+      rw[<-mrg.sym.static]; assumption
     | im _ _ mrg =>
-      have ⟨Δa', Δb', mrg, agr1, agr2⟩ := ih mrg
+      have ⟨Δa', Δb', _, agr1, agr2⟩ := ih mrg
       existsi A.[σ] :⟨.im, s⟩ Δa', A.[σ] :⟨.im, s⟩ Δb'; and_intros
-      all_goals constructor <;> assumption
+      all_goals constructor <;> try assumption
+      rw[<-mrg.static]; assumption
+      rw[<-mrg.sym.static]; assumption
   case intro_im agr ih =>
     cases mrg with
     | im _ _ mrg =>
       have ⟨Δa', Δb', mrg, agr1, agr2⟩ := ih mrg
       existsi Δa', Δb'; and_intros
       . assumption
-      . constructor <;> assumption
-      . constructor <;> assumption
+      . constructor <;> try assumption
+        rw[<-mrg.static]; assumption
+      . constructor <;> try assumption
+        rw[<-mrg.sym.static]; assumption
   case intro_ex mrg1 lw tym agr ih =>
     cases mrg with
     | contra _ _ h mrg =>
@@ -173,7 +183,10 @@ lemma AgreeSubst.split {Γ Γ'} {Δ Δ' Δa Δb : Ctx Srt} {σ σ'} :
         . exact tym
         . exact agr1
       . apply AgreeSubst.intro_im
-        . exact tym.toStatic
+        . rw[<-mrg2.sym.static]
+          rw[<-mrg1.sym.static]
+          rw[mrg1.static]
+          exact tym.toStatic
         . exact agr2
     | right _ _ mrg =>
       have ⟨Δa', Δb', mrg2, agr1, agr2⟩ := ih mrg
@@ -181,7 +194,10 @@ lemma AgreeSubst.split {Γ Γ'} {Δ Δ' Δa Δb : Ctx Srt} {σ σ'} :
       existsi Δa', Δc1; and_intros
       . exact mrg4.sym
       . apply AgreeSubst.intro_im
-        . exact tym.toStatic
+        . rw[<-mrg2.static]
+          rw[<-mrg1.sym.static]
+          rw[mrg1.static]
+          exact tym.toStatic
         . exact agr1
       . apply AgreeSubst.intro_ex
         . exact mrg3.sym
@@ -192,27 +208,69 @@ lemma AgreeSubst.split {Γ Γ'} {Δ Δ' Δa Δb : Ctx Srt} {σ σ'} :
     cases mrg with
     | contra _ _ h mrg =>
       have ⟨Δa', Δb', mrg', agr1, agr2⟩ := ih (Merge.contra A s h mrg)
-      existsi Δa', Δb'; aesop (rule_sets := [subst])
+      existsi Δa', Δb'; and_intros
+      . assumption
+      . constructor
+        assumption
+        rw[<-mrg.static]; assumption
+        rw[<-mrg'.static]; assumption
+        assumption
+      . constructor
+        assumption
+        rw[<-mrg.sym.static]; assumption
+        rw[<-mrg'.sym.static]; assumption
+        assumption
     | left _ _ mrg =>
       have ⟨Δa', Δb', mrg', agr1, agr2⟩ := ih (Merge.left A s mrg)
-      existsi Δa', Δb'; aesop (rule_sets := [subst])
+      existsi Δa', Δb'; and_intros
+      . assumption
+      . constructor
+        assumption
+        rw[<-mrg.static]; assumption
+        rw[<-mrg'.static]; assumption
+        assumption
+      . constructor
+        assumption
+        rw[<-mrg.sym.static]; assumption
+        rw[<-mrg'.sym.static]; assumption
+        assumption
     | right _ _ mrg =>
       have ⟨Δa', Δb', mrg', agr1, agr2⟩ := ih (Merge.right A s mrg)
-      existsi Δa', Δb'; aesop (rule_sets := [subst])
+      existsi Δa', Δb'; and_intros
+      . assumption
+      . constructor
+        assumption
+        rw[<-mrg.static]; assumption
+        rw[<-mrg'.static]; assumption
+        assumption
+      . constructor
+        assumption
+        rw[<-mrg.sym.static]; assumption
+        rw[<-mrg'.sym.static]; assumption
+        assumption
     | im _ _ mrg =>
       have ⟨Δa', Δb', mrg', agr1, agr2⟩ := ih (Merge.im _ _ mrg)
-      existsi Δa', Δb'; aesop (rule_sets := [subst])
+      existsi Δa', Δb'; and_intros
+      . assumption
+      . constructor
+        assumption
+        rw[<-mrg.static]; assumption
+        rw[<-mrg'.static]; assumption
+        assumption
+      . constructor
+        assumption
+        rw[<-mrg.sym.static]; assumption
+        rw[<-mrg'.sym.static]; assumption
+        assumption
 
 @[aesop safe (rule_sets := [subst])]
-lemma AgreeSubst.wf {Γ Γ'} {Δ Δ' : Ctx Srt} {σ σ'} :
-    AgreeSubst σ σ' Γ Δ Γ' Δ' ->
-    Γ ;; Δ ⊢ -> Γ' ;; Δ' ⊢ := by
+lemma AgreeSubst.wf {Δ Δ' : Ctx Srt} {σ σ'} :
+    AgreeSubst σ σ' Δ Δ' -> Δ ⊢ -> Δ' ⊢ := by
   intro agr; apply agr.toDynamic.wf
 
-lemma Erased.substitution {Γ Γ'} {Δ Δ' : Ctx Srt} {A m m' σ σ'} :
-    Γ ;; Δ ⊢ m ▷ m' : A -> AgreeSubst σ σ' Γ Δ Γ' Δ' ->
-    Γ' ;; Δ' ⊢ m.[σ] ▷ m'.[σ'] : A.[σ] := by
-  intro ty agr; induction ty generalizing Γ' Δ' σ σ' <;> asimp
+lemma Erased.substitution {Δ Δ' : Ctx Srt} {A m m' σ σ'} :
+    Δ ⊢ m ▷ m' :: A -> AgreeSubst σ σ' Δ Δ' -> Δ' ⊢ m.[σ] ▷ m'.[σ'] :: A.[σ] := by
+  intro ty agr; induction ty generalizing Δ' σ σ' <;> asimp
   case var wf hs =>
     apply agr.has (agr.wf wf) hs
   case lam_im lw tyA erm ihm =>
@@ -310,10 +368,10 @@ lemma Erased.substitution {Γ Γ'} {Δ Δ' : Ctx Srt} {A m m' σ σ'} :
     . assumption
     . assumption
 
-lemma Erased.subst_im {Γ} {Δ : Ctx Srt} {A B m m' n s} :
-    A :: Γ ;; A :⟨.im, s⟩ Δ ⊢ m ▷ m' : B ->
-    Γ ⊢ n : A ->
-    Γ ;; Δ ⊢ m.[n/] ▷ m'.[.null/] : B.[n/] := by
+lemma Erased.subst_im {Δ : Ctx Srt} {A B m m' n s} :
+    A :⟨.im, s⟩ Δ ⊢ m ▷ m' :: B ->
+    Δ.static ⊢ n : A ->
+    Δ ⊢ m.[n/] ▷ m'.[.null/] :: B.[n/] := by
   intro erm tyn
   obtain ⟨_, _, _⟩ := erm.ctx_inv
   apply erm.substitution
@@ -321,11 +379,11 @@ lemma Erased.subst_im {Γ} {Δ : Ctx Srt} {A B m m' n s} :
   . asimp; assumption
   . apply AgreeSubst.refl; assumption
 
-lemma Erased.subst_ex {Γ} {Δ1 Δ2 Δ : Ctx Srt} {A B m m' n n' s} :
+lemma Erased.subst_ex {Δ1 Δ2 Δ : Ctx Srt} {A B m m' n n' s} :
     Lower Δ2 s -> Merge Δ1 Δ2 Δ ->
-    A :: Γ ;; A :⟨.ex, s⟩ Δ1 ⊢ m ▷ m' : B ->
-    Γ ;; Δ2 ⊢ n ▷ n' : A ->
-    Γ ;; Δ ⊢ m.[n/] ▷ m'.[n'/] : B.[n/] := by
+    A :⟨.ex, s⟩ Δ1 ⊢ m ▷ m' :: B ->
+    Δ2 ⊢ n ▷ n' :: A ->
+    Δ ⊢ m.[n/] ▷ m'.[n'/] :: B.[n/] := by
   intro lw mrg tym tyn
   obtain ⟨_, _, _⟩ := tym.ctx_inv
   apply tym.substitution
@@ -335,33 +393,33 @@ lemma Erased.subst_ex {Γ} {Δ1 Δ2 Δ : Ctx Srt} {A B m m' n n' s} :
   . asimp; assumption
   . apply AgreeSubst.refl; assumption
 
-lemma Erased.esubst_im {Γ} {Δ : Ctx Srt} {A B1 B2 m1 m2 e1 e2 n s} :
+lemma Erased.esubst_im {Δ : Ctx Srt} {A B1 B2 m1 m2 e1 e2 n s} :
     m2 = m1.[n/] ->
     e2 = e1.[.null/] ->
     B2 = B1.[n/] ->
-    A :: Γ ;; A :⟨.im, s⟩ Δ ⊢ m1 ▷ e1 : B1 ->
-    Γ ⊢ n : A ->
-    Γ ;; Δ ⊢ m2 ▷ e2 : B2 := by
+    A :⟨.im, s⟩ Δ ⊢ m1 ▷ e1 :: B1 ->
+    Δ.static ⊢ n : A ->
+    Δ ⊢ m2 ▷ e2 :: B2 := by
   intros; subst_vars; apply Erased.subst_im <;> assumption
 
-lemma Erased.esubst_ex {Γ} {Δ1 Δ2 Δ : Ctx Srt} {A B1 B2 m1 e1 m2 e2 n1 n2 s} :
+lemma Erased.esubst_ex {Δ1 Δ2 Δ : Ctx Srt} {A B1 B2 m1 e1 m2 e2 n1 n2 s} :
     m2 = m1.[n1/] ->
     e2 = e1.[n2/] ->
     B2 = B1.[n1/] ->
     Lower Δ2 s -> Merge Δ1 Δ2 Δ ->
-    A :: Γ ;; A :⟨.ex, s⟩ Δ1 ⊢ m1 ▷ e1 : B1 ->
-    Γ ;; Δ2 ⊢ n1 ▷ n2 : A ->
-    Γ ;; Δ ⊢ m2 ▷ e2 : B2 := by
+    A :⟨.ex, s⟩ Δ1 ⊢ m1 ▷ e1 :: B1 ->
+    Δ2 ⊢ n1 ▷ n2 :: A ->
+    Δ ⊢ m2 ▷ e2 :: B2 := by
   intros; subst_vars; apply Erased.subst_ex <;> assumption
 
-lemma Erased.conv_ctx {Γ} {Δ : Ctx Srt} {A B C m m' r s i} :
+lemma Erased.conv_ctx {Δ : Ctx Srt} {A B C m m' r s i} :
     B === A ->
-    Γ ⊢ B : .srt s i ->
-    A :: Γ ;; A :⟨r, s⟩ Δ ⊢ m ▷ m' : C ->
-    B :: Γ ;; B :⟨r, s⟩ Δ ⊢ m ▷ m' : C := by
+    Δ.static ⊢ B : .srt s i ->
+    A :⟨r, s⟩ Δ ⊢ m ▷ m' :: C ->
+    B :⟨r, s⟩ Δ ⊢ m ▷ m' :: C := by
   intro eq tyB erm
   obtain ⟨_, wf, tyA⟩ := erm.ctx_inv
-  replace erm : B :: Γ ;; B :⟨r, s⟩ Δ ⊢ m.[ids] ▷ m'.[ids] : C.[ids] := by
+  replace erm : B :⟨r, s⟩ Δ ⊢ m.[ids] ▷ m'.[ids] :: C.[ids] := by
     apply erm.substitution
     apply AgreeSubst.conv <;> try assumption
     . asimp; apply tyA.weaken tyB
