SStructTT/SStruct/Dynamic/Progress.lean
@@ -7,10 +7,9 @@ namespace SStruct.Dynamic
 variable {Srt : Type} [ord : SrtOrder Srt]
 
 lemma Typed.pi_canonical {A B C m : Tm Srt} {r s} :
-    [] ;; [] ⊢ m : C -> C === .pi A B r s -> Value m ->
+    [] ⊢ m :: C -> C === .pi A B r s -> Value m ->
     ∃ A n, m = .lam A n r s := by
-  generalize e1: [] = Γ
-  generalize e2: [] = Δ
+  generalize e: [] = Δ
   intro ty eq vl; induction ty <;> try trivial
   all_goals try false_conv
   case lam_im A B m _ _ _ _ _ _ _  =>
@@ -26,10 +25,9 @@ lemma Typed.pi_canonical {A B C m : Tm Srt} {r s} :
     apply Conv.trans <;> assumption
 
 lemma Typed.sig_canonical {A B C m : Tm Srt} {r s} :
-    [] ;; [] ⊢ m : C -> C === .sig A B r s -> Value m ->
+    [] ⊢ m :: C -> C === .sig A B r s -> Value m ->
     ∃ m1 m2, m = .tup m1 m2 r s := by
-  generalize e1: [] = Γ
-  generalize e2: [] = Δ
+  generalize e: [] = Δ
   intro ty eq vl; induction ty <;> try trivial
   all_goals try false_conv
   case tup_im A0 B0 m n _ _ _ _ _ _ =>
@@ -45,9 +43,8 @@ lemma Typed.sig_canonical {A B C m : Tm Srt} {r s} :
     apply Conv.trans <;> assumption
 
 lemma Typed.bool_canonical {C m : Tm Srt} :
-    [] ;; [] ⊢ m : C -> C === .bool -> Value m -> m = .tt ∨ m = .ff := by
-  generalize e1: [] = Γ
-  generalize e2: [] = Γ
+    [] ⊢ m :: C -> C === .bool -> Value m -> m = .tt ∨ m = .ff := by
+  generalize e: [] = Δ
   intro ty eq vl; induction ty <;> try trivial
   all_goals try false_conv
   case tt => simp
@@ -59,9 +56,8 @@ lemma Typed.bool_canonical {C m : Tm Srt} :
     apply Conv.trans <;> assumption
 
 lemma Typed.idn_canonical {A C m a b : Tm Srt} :
-    [] ;; [] ⊢ m : C -> C === .idn A a b -> Value m -> ∃ n, m = .rfl n := by
-  generalize e1: [] = Γ
-  generalize e2: [] = Δ
+    [] ⊢ m :: C -> C === .idn A a b -> Value m -> ∃ n, m = .rfl n := by
+  generalize e: [] = Δ
   intro ty eq vl; induction ty <;> try trivial
   all_goals try false_conv
   case drop mrg _ _ _ _ =>
@@ -71,13 +67,12 @@ lemma Typed.idn_canonical {A C m a b : Tm Srt} :
     apply Conv.trans <;> assumption
 
 theorem Typed.progress {m A : Tm Srt} :
-    [] ;; [] ⊢ m : A -> (∃ n, m ~>> n) ∨ Value m := by
-  generalize e1: [] = Γ
-  generalize e2: [] = Δ
+    [] ⊢ m :: A -> (∃ n, m ~>> n) ∨ Value m := by
+  generalize e: [] = Δ
   intro ty; induction ty <;> (subst_vars; simp_all; try trivial)
   case lam_im => right; constructor
   case lam_ex => right; constructor
-  case app_im n _ _ tym ih =>
+  case app_im n _ tym tyn ih =>
     match ih with
     | .inl ⟨m, _⟩ =>
       left; existsi Tm.app m n .im
@@ -106,7 +101,7 @@ theorem Typed.progress {m A : Tm Srt} :
       left; existsi Tm.tup m n .im s
       constructor; assumption
     | .inr _ => right; constructor; assumption
-  case tup_ex m n s _ _ _ _ ihm ihn mrg =>
+  case tup_ex m n s _ _ _ ihm ihn mrg ty =>
     cases mrg; simp_all
     match ihm with
     | .inl ⟨m, _⟩ =>
@@ -118,7 +113,7 @@ theorem Typed.progress {m A : Tm Srt} :
         left; existsi Tm.tup m n .ex s
         constructor; assumption
       | .inr _ => right; constructor <;> assumption
-  case prj_im C _ n _ _ _ _ _ _ tym _ ihm mrg =>
+  case prj_im C _ n _ _ _ _ _ tym ihn ihm mrg tyC =>
     cases mrg; simp_all
     match ihm with
     | .inl ⟨m, _⟩ =>
@@ -128,7 +123,7 @@ theorem Typed.progress {m A : Tm Srt} :
       have ⟨m1, m2, _⟩ := tym.sig_canonical Conv.R vl
       subst_vars; left; existsi n.[m2,m1/]
       constructor; assumption
-  case prj_ex C _ n _ _ _ _ _ _ tym _ ihm mrg =>
+  case prj_ex C _ n _ _ _ _ _ tym ihn ihm mrg tyC =>
     cases mrg; simp_all
     match ihm with
     | .inl ⟨m, _⟩ =>
@@ -140,7 +135,7 @@ theorem Typed.progress {m A : Tm Srt} :
       constructor; assumption
   case tt => right; constructor
   case ff => right; constructor
-  case ite A _ n1 n2 _ _ _ tym _ _ ihm _ _ mrg =>
+  case ite A m n1 n2 _ _ tym _ _ ihm _ _ mrg _ =>
     cases mrg; simp_all
     match ihm with
     | .inl ⟨m, _⟩ =>
